\begin{equation}
\begin{split}
    \lim_{x \to a} \Big[ f(x) + g(x) \Big] &= \lim_{x \to a} f(x) + \lim_{x \to a} g(x) \\
    \lim_{x \to a} \Big[ f(x) - g(x) \Big] &= \lim_{x \to a} f(x) - \lim_{x \to a} g(x) \\
    \lim_{x \to a} \Big[ c \cdot f(x) \Big] &= c \cdot \lim_{x \to a} f(x) \\
    \lim_{x \to a} \Big[ f(x) \cdot g(x) \Big] &= \lim_{x \to a} f(x) \cdot \lim_{x \to a} g(x) \\
    \lim_{x \to a} \frac{f(x)}{g(x)} &= \frac{\lim_{x \to a} f(x)}{\lim_{x \to a}g(x)} \; \text{if} \lim_{x \to a}g(x) \neq 0
\end{split}
\end{equation}